aeneas-lean/Tree.lean
@@ -18,6 +18,7 @@ import Tree.ProgressiveList.ApplyUpdates.Contents
 import Tree.ProgressiveList.Mutable
 import Tree.ProgressiveList.Spine
 import Tree.ProgressiveList.CopyOnWrite
+import Tree.Cow.Metadata
 import Tree.PackedLeaf.Contents
 import Tree.PackedLeaf.BulkUpdate
 import Tree.BulkUpdate
