aeneas-lean/Tree/Types.lean
@@ -270,7 +270,7 @@ structure cow.CowOnMut where
   max_index : Option (update_map.MaxIndexState × Std.Usize)
 
 /-- [milhouse::cow::VecCow]
-    Source: 'src/cow.rs', lines 135:0-143:1
+    Source: 'src/cow.rs', lines 138:0-146:1
     Visibility: public -/
 @[discriminant isize]
 inductive cow.VecCow (T : Type) where
@@ -278,7 +278,7 @@ inductive cow.VecCow (T : Type) where
 | Mutable : T → cow.VecCow T
 
 /-- [milhouse::cow::BTreeCow]
-    Source: 'src/cow.rs', lines 87:0-95:1
+    Source: 'src/cow.rs', lines 90:0-98:1
     Visibility: public -/
 @[discriminant isize]
 inductive cow.BTreeCow (T : Type) where
@@ -289,7 +289,7 @@ inductive cow.BTreeCow (T : Type) where
 | Mutable : T → cow.BTreeCow T
 
 /-- [milhouse::cow::Cow]
-    Source: 'src/cow.rs', lines 24:0-27:1
+    Source: 'src/cow.rs', lines 27:0-30:1
     Visibility: public -/
 @[discriminant isize]
 inductive cow.Cow (T : Type) where
